Setting up the erasure.

concurrency/erasure.v
@@ -1,5 +1,102 @@
 
-Add LoadPath "../compcomp" as compcomp.
+Add LoadPath "../concurrency" as concurrency.
 
+Require Import Memory.
+
+(* The concurrent machinery*)
 Require Import concurrent_machine.
+Require Import juicy_machine. Import Concur.
+Require Import compcert_threads. Import Concur.
 
+(*The simulations*)
+Require Import wholeprog_simulations. 
+
+Module Erasure (SCH: Scheduler NatTID)(SEM: Semantics).
+  Import SEM.
+  Parameter genv: G.
+  Parameter main: Values.val.
+    
+  Module JSEM:= JuicyMachineSig SEM.
+  Module JuicyMachine:= CoarseMachine NatTID SCH JSEM.
+  Definition JMachineSem:= JuicyMachine.MachineSemantics.
+  
+  Module DSEM:= ShareMachineSig SEM.
+  Module DryMachine:= CoarseMachine NatTID SCH DSEM.
+  Definition DMachineSem:= DryMachine.MachineSemantics.
+
+  (* The main erasure theorem is stated with Wholeprog_sim
+     which might change, but will escentially have the same
+     structure: match, init_clause, core_diagram, etc...  *)
+  Definition ge_inv (g1 g2: SEM.G):= g1 = g2.
+  Inductive init_inv:  Values.Val.meminj ->
+                       G -> list Values.val -> mem ->
+                       G -> list Values.val -> mem -> Prop:=
+  |InitEq: forall j g1 args1 m1 g2 args2 m2,
+      g1 = g2 ->
+      args1 = args2 ->
+      m1 = m2 ->
+      init_inv j g1 args1 m1 g2 args2 m2.
+
+  Inductive halt_inv:  SM_Injection ->
+                       G -> Values.val -> mem ->
+                       G -> Values.val -> mem -> Prop:=
+  |HaltEq: forall j g1 args1 m1 g2 args2 m2,
+      g1 = g2 ->
+      args1 = args2 ->
+      m1 = m2 ->
+      halt_inv j g1 args1 m1 g2 args2 m2.
+
+  Definition core_data:= unit.
+  Definition match_state (d: core_data) (j: SM_Injection)
+             (JS: JuicyMachine.MachState)(M1: mem)
+             (DS: DryMachine.MachState)(M2: mem):= True.
+  Definition core_ord: unit-> unit -> Prop := fun _ _ => False.
+  Definition core_ord_wf:  well_founded core_ord.
+      constructor; intros y H; inversion H.
+  Defined.
+  Lemma core_initial (j: Values.Val.meminj)
+             (JS: JuicyMachine.MachState)(vals1:list Values.val)(m1: mem)
+             (vals2:list Values.val)(m2: mem)
+             : initial_core JMachineSem genv main vals1 = Some JS ->
+                   init_inv j genv vals1 m1 genv vals2 m2 ->
+                   exists (mu : SM_Injection) (cd : core_data) 
+                   (DS : DryMachine.MachState),
+                     as_inj mu = j /\
+                     initial_core DMachineSem genv main vals2 = Some DS /\
+                     match_state cd mu JS m1 DS m2.
+  Proof.
+    intros INIT_C INIT_INV.
+    inversion INIT_INV; subst.
+    pose (mu:=(initial_SM
+         (fun _ : block => false)(fun _ : block => false)
+         (fun b:block => match j b with Some _ => true | None => false end)
+         (fun b:block => match j b with Some _ => true | None => false end)
+         j)).
+    
+    exists mu, tt.
+    admit.
+    (*eexists. (* Fill in! *)
+    split.
+    unfold mu; apply initial_SM_as_inj.
+    split.
+    unfold initial_core, DMachineSem,  DryMachine.MachineSemantics.
+    unfold DryMachine.init_machine.
+     *)
+    Qed.
+    
+    Theorem erasure:
+    Wholeprog_sim.Wholeprog_sim
+      JMachineSem DMachineSem
+      genv genv
+      main
+      ge_inv init_inv halt_inv.
+      apply (Wholeprog_sim.Build_Wholeprog_sim
+            JMachineSem DMachineSem
+            genv genv
+            main
+            ge_inv init_inv halt_inv
+            core_data match_state core_ord core_ord_wf).
+      - reflexivity.
+      - apply core_initial.                                                         -          
+
+  
